HoareLogic/SimpleSmallStepSemantics.v
@@ -3,11 +3,11 @@ Require Import Logic.SeparationLogic.Model.SeparationAlgebra.
 Require Import Logic.HoareLogic.ImperativeLanguage.
 Require Import Logic.HoareLogic.ProgramState.
 
-Class SimpleSmallStepSemantics (P: ProgrammingLanguage) (state: Type): Type := {
+Class SimpleSmallStepSemantics cmd {P: ProgrammingLanguage cmd} (state: Type): Type := {
   simple_step: cmd * state -> cmd * state -> Prop
 }.
 
-Definition step {P: ProgrammingLanguage} {state: Type} {SSSS: SimpleSmallStepSemantics P state} (final_state: cmd * state -> Prop) (cs: cmd * state) (mcs: MetaState (cmd * state)) :=
+Definition step {cmd} {P: ProgrammingLanguage cmd} {state: Type} {SSSS: SimpleSmallStepSemantics cmd state} (final_state: cmd * state -> Prop) (cs: cmd * state) (mcs: MetaState (cmd * state)) :=
   match mcs with
   | Terminating cs0 => simple_step cs cs0
   | NonTerminating => False
